Initial commit Verify client.dfy (#300)
* Verification and restructuring basic proof

feat: Added correct key added
chore: Added more extensive frames prover
chore: Added ghost return frame variable

* Added signature verification

* Moved Predicates to correct files added start signature CMM

* Finished Encrypt verification

chore: Removed all requirements which where not part of the client from the client
chore: Added part of the verification to the corresponding files

* Refactoring encrypt to accomodate duality decrypt

* Simplified sorting

* Added duality serialize and deserialize one pair

Updated proof deserialize kvPair by proving serialize instead

* Created Definition LinearSeqToMap

Created new definition LinearSeqToMap and proved duality MapToLinear

* Finished Proof DeserializeAAD and cleanup

feat: added proof DeserializeAAD

* Added proofs all fields of header body

feat: Added predicates and proofs MessageHeaderBody and MessageHeader
feat: Added prove duality MessageHeaderBody serialize and deserialize

* Added two assert statements to allow validation of unrelated code

* Added base post condition Client decrypt

* Solved verification decrypt problems

* Added base proof that correct key is used for encryption

* Added opaque lemmas

src/SDK/CMM/Defs.dfy
@@ -25,8 +25,10 @@ module {:extern "CMMDefs"} CMMDefs {
                                   returns (res: Result<Materials.ValidEncryptionMaterials>)
       requires Valid()
       modifies Repr
+      ensures Valid()
+      ensures res.Success? ==> EncryptionMaterialsSignature(res.value)
+      ensures res.Success? ==> res.value.plaintextDataKey.Some? && res.value.Serializable()
       ensures Valid() && fresh(Repr - old(Repr))
-      ensures res.Success? ==> res.value.Serializable()
 
     // The following predicate is a synonym for Encryption.Serializable and provides a workaround for a translation bug
     // of "fuel" in trait-override checks in Dafny. https://github.com/dafny-lang/dafny/issues/422
@@ -41,4 +43,16 @@ module {:extern "CMMDefs"} CMMDefs {
       ensures Valid() && fresh(Repr - old(Repr))
       ensures res.Success? ==> res.value.plaintextDataKey.Some?
   }
+
+  // Predicate works arround a known error in Dafny: https://github.com/dafny-lang/dafny/issues/422 
+  predicate EncryptionMaterialsSignature(validEncryptionMaterials: Materials.ValidEncryptionMaterials) {
+    EncryptionMaterialsSignatureOpaque(validEncryptionMaterials)
+  }
+
+  predicate {:opaque } EncryptionMaterialsSignatureOpaque(validEncryptionMaterials: Materials.ValidEncryptionMaterials)
+  {
+    true
+  }
+
+
 }
